Stage work on vsubterm_agree_upto_thm

examples/lambda/barendregt/separabilityScript.sml
@@ -2794,8 +2794,8 @@ Definition Boehm_construction' :
     let n_max = MAX_LIST (MAP (\e. subterm_length e p) Ms);
         d_max = MAX_LIST (MAP (\e. vsubterm_width e p) Ms) + n_max;
         k     = LENGTH Ms;
-        X'    = BIGUNION (IMAGE FV (set Ms));
-        vs0   = NEWS (n_max + SUC d_max + k) (X UNION X');
+        Y    = BIGUNION (IMAGE FV (set Ms));
+        vs0   = NEWS (n_max + SUC d_max + k) (X UNION Y);
         vs    = TAKE n_max vs0;
         xs    = DROP n_max vs0;
         M0 i  = principal_hnf (EL i Ms);
@@ -2833,7 +2833,8 @@ Proof
  >> Q.X_GEN_TAC ‘N’
  >> DISCH_TAC
  >> UNBETA_TAC [Boehm_construction'] “Boehm_construction' X Ms' p”
- >> qunabbrev_tac ‘X'’
+ (* re-define Y *)
+ >> qunabbrev_tac ‘Y'’
  >> qabbrev_tac ‘Y = BIGUNION (IMAGE FV (set Ms'))’
  >> ‘FINITE Y’ by (rw [Abbr ‘Y’] >> rw [])
  >> simp [Boehm_apply_APPEND]
@@ -7630,6 +7631,7 @@ Proof
  >> FIRST_X_ASSUM MATCH_MP_TAC >> art []
 QED
 
+(* cf. agree_upto_def *)
 Definition vsubterm_agree_upto_def :
     vsubterm_agree_upto X Ms p r <=>
     !q M N. q <<= p /\ q <> p /\ MEM M Ms /\ MEM N Ms /\
@@ -7638,14 +7640,18 @@ Definition vsubterm_agree_upto_def :
             equivalent (vsubterm' X M q r) (vsubterm' X N q r)
 End
 
+(* cf. agree_upto_lemma *)
 Theorem vsubterm_agree_upto_lemma :
     !X Ms p r. FINITE X /\ p <> [] /\ 0 < r /\
-               vsubterm_agree_upto X Ms p r /\
-              (!M. MEM M Ms ==> FV M SUBSET X UNION RANK r) ==>
+              (!M. MEM M Ms ==> FV M SUBSET X UNION RANK r) /\
+               vsubterm_agree_upto X Ms p r ==>
        ?pi. Boehm_transform pi /\
            (!M. MEM M Ms ==> FV (apply pi M) SUBSET X UNION RANK r) /\
            (!M. MEM M Ms ==> is_ready (apply pi M)) /\
             vsubterm_agree_upto X (apply pi Ms) p r /\
+           (!q M. MEM M Ms /\ q <<= p ==>
+                 (vsubterm X M q r = NONE <=>
+                  vsubterm X (apply pi M) q r = NONE)) /\
            (!M. MEM M Ms /\ vsubterm X M p r <> NONE ==>
                (solvable (vsubterm' X M p r) <=>
                 solvable (vsubterm' X (apply pi M) p r))) /\
@@ -7669,6 +7675,424 @@ Proof
  >> ‘vsubterm X M q r <> NONE /\ vsubterm X N q r <> NONE’ by PROVE_TAC []
  >> ‘equivalent (vsubterm' X M q r) (vsubterm' X N q r)’ by PROVE_TAC []
  >> PROVE_TAC []
+QED
+
+(* cf. faithful_def *)
+Definition vsubterm_faithful_def :
+    vsubterm_faithful p X Ms pi r <=>
+      (!M. MEM M Ms /\ vsubterm X M p r <> NONE ==>
+          (solvable (vsubterm' X M p r) <=>
+           solvable (apply pi M))) /\
+      (!M N. MEM M Ms /\ MEM N Ms /\
+             vsubterm X M p r <> NONE /\
+             vsubterm X N p r <> NONE ==>
+            (equivalent (vsubterm' X M p r) (vsubterm' X N p r) <=>
+             equivalent (apply pi M) (apply pi N)))
+End
+
+Theorem vsubterm_faithful_two :
+   !p X M N pi r.
+       vsubterm_faithful p X [M; N] pi r <=>
+      (vsubterm X M p r <> NONE ==> (solvable (vsubterm' X M p r) <=>
+                                     solvable (apply pi M))) /\
+      (vsubterm X N p r <> NONE ==> (solvable (vsubterm' X N p r) <=>
+                                     solvable (apply pi N))) /\
+      (vsubterm X M p r <> NONE /\
+       vsubterm X N p r <> NONE ==> (equivalent (vsubterm' X M p r)
+                                                (vsubterm' X N p r) <=>
+                                     equivalent (apply pi M) (apply pi N)))
+Proof
+    rpt STRIP_TAC
+ >> EQ_TAC >> rw [vsubterm_faithful_def] >> gs []
+ >> PROVE_TAC [equivalent_comm]
+QED
+
+Overload vsubterm_faithful' = “vsubterm_faithful []”
+
+(* |- !X Ms pi r.
+        vsubterm_faithful' X Ms pi r <=>
+        (!M. MEM M Ms ==> (solvable M <=> solvable (apply pi M))) /\
+        !M N.
+          MEM M Ms /\ MEM N Ms ==>
+          (equivalent M N <=> equivalent (apply pi M) (apply pi N))
+ *)
+Theorem vsubterm_faithful' =
+        vsubterm_faithful_def |> Q.SPEC ‘[]’ |> SRULE []
+
+(* |- !X M N pi r.
+        vsubterm_faithful' X [M; N] pi r <=>
+        (solvable M <=> solvable (apply pi M)) /\
+        (solvable N <=> solvable (apply pi N)) /\
+        (equivalent M N <=> equivalent (apply pi M) (apply pi N))
+ *)
+Theorem vsubterm_faithful_two' =
+        vsubterm_faithful_two |> Q.SPEC ‘[]’ |> SRULE []
+
+(* cf. agree_upto_thm *)
+Theorem vsubterm_agree_upto_thm :
+    !X Ms p r. FINITE X /\ 0 < r /\
+              (!M. MEM M Ms ==> FV M SUBSET X UNION RANK r) /\
+               vsubterm_agree_upto X Ms p r ==>
+               ?pi. Boehm_transform pi /\ vsubterm_faithful p X Ms pi r
+Proof
+    rpt GEN_TAC
+ (* push ‘FINITE X’ to assumption *)
+ >> Cases_on ‘FINITE X’ >> simp []
+ (* preparing for induction *)
+ >> qid_specl_tac [‘p’, ‘Ms’, ‘r’]
+ >> Induct_on ‘p’
+ >- (rpt STRIP_TAC \\
+     Q.EXISTS_TAC ‘[]’ >> simp [vsubterm_faithful'])
+ (* stage work *)
+ >> rw [vsubterm_faithful_def]
+ >> cheat
+ (* TODO
+ (* trivial case: all unsolvable *)
+ >> Cases_on ‘!M. MEM M Ms ==> unsolvable M’
+ >- (Q.EXISTS_TAC ‘[]’ \\
+     reverse (rw [])
+     >- (rw [equivalent_of_unsolvables] \\
+         rw [subtree_equiv_def, BT_of_unsolvables]) \\
+     MP_TAC (Q.SPECL [‘X’, ‘M’, ‘r’] BT_valid_paths_thm') >> rw [] \\
+     Know ‘subterm X M (h::p) r = NONE <=> h::p NOTIN ltree_paths (BT' X M r)’
+     >- (Suff ‘h::p IN ltree_paths (BT' X M r) <=> subterm X M (h::p) r <> NONE’
+         >- PROVE_TAC [] \\
+         MATCH_MP_TAC BT_ltree_paths_thm >> simp []) >> Rewr' \\
+     STRONG_DISJ_TAC \\
+     Suff ‘solvable M’ >- METIS_TAC [] \\
+     MATCH_MP_TAC ltree_paths_imp_solvable \\
+     qexistsl_tac [‘h::p’, ‘X’, ‘r’] >> simp [])
+ (* one is solvable, all are solvable *)
+ >> Know ‘!M. MEM M Ms ==> solvable M’
+ >- (rpt STRIP_TAC \\
+     MATCH_MP_TAC ltree_paths_imp_solvable \\
+     qexistsl_tac [‘h::p’, ‘X’, ‘r’] >> simp [GSYM BT_paths_thm])
+ >> POP_ASSUM K_TAC >> DISCH_TAC
+ (* applying agree_upto_lemma *)
+ >> MP_TAC (Q.SPECL [‘X’, ‘Ms’, ‘h::p’, ‘r’] agree_upto_lemma) >> rw []
+ (* p0 is asserted *)
+ >> rename1 ‘Boehm_transform p0’
+ >> fs [is_ready_alt']
+ (* decomposing Ms *)
+ >> qabbrev_tac ‘k = LENGTH Ms’
+ >> ‘k <> 0’ by rw [Abbr ‘k’, LENGTH_NIL]
+ >> qabbrev_tac ‘M = \i. EL i Ms’
+ >> Know ‘!P. (!N. MEM N Ms ==> P N) <=> !i. i < k ==> P (M i)’
+ >- (Q.X_GEN_TAC ‘P’ \\
+     reverse EQ_TAC >> rw [MEM_EL] >- simp [] \\
+     FIRST_X_ASSUM MATCH_MP_TAC \\
+     Q.EXISTS_TAC ‘i’ >> art [])
+ >> DISCH_THEN (fs o wrap)
+ >> qabbrev_tac ‘M1 = \i. principal_hnf (apply p0 (M i))’
+ >> Know ‘!i. i < k ==> ?y Ns. M1 i = VAR y @* Ns /\ EVERY (\e. y # e) Ns’
+ >- (rpt STRIP_TAC \\
+     Q.PAT_X_ASSUM ‘!i. i < k ==> solvable (apply p0 (M i)) /\ _’ drule \\
+     rw [Abbr ‘M1’] \\
+     qexistsl_tac [‘y’, ‘Ns’] >> art [] \\
+     rw [principal_hnf_thm', hnf_appstar])
+ >> DISCH_TAC
+ (* NOTE: take the head variable and children terms from ‘N 0’ *)
+ >> Know ‘?y Ns. M1 0 = VAR y @* Ns’
+ >- (POP_ASSUM (MP_TAC o Q.SPEC ‘0’) >> rw [] \\
+     qexistsl_tac [‘y’, ‘Ns’] >> art [])
+ >> STRIP_TAC
+ >> qabbrev_tac ‘m = LENGTH Ns’
+ >> Know ‘!i. i < k ==> ?Ns. M1 i = VAR y @* Ns /\ EVERY (\e. y # e) Ns /\
+                             LENGTH Ns = m’
+ >- (rpt STRIP_TAC \\
+     Q.PAT_X_ASSUM ‘!i. i < k ==> ?y Ns. P’ drule >> rw [] \\
+     Q.EXISTS_TAC ‘Ns'’ \\
+     Suff ‘y = y' /\ LENGTH Ns' = m’ >- rw [] \\
+     Cases_on ‘i = 0’ >- fs [] \\
+     FULL_SIMP_TAC std_ss [agree_upto_def] \\
+     Q.PAT_X_ASSUM ‘!q M N. q <<= h::p /\ q <> h::p /\
+                            MEM M (apply p0 Ms) /\ _ ==> _’
+       (MP_TAC o Q.SPECL [‘[]’, ‘apply p0 ((M :num -> term) 0)’,
+                                ‘apply p0 ((M :num -> term) i)’]) \\
+     simp [subtree_equiv_def, MEM_MAP] \\
+     impl_tac
+     >- (CONJ_TAC >| (* 2 subgoals *)
+         [ (* goal 1 (of 2) *)
+           Q.EXISTS_TAC ‘M 0’ >> simp [MEM_EL] \\
+           Q.EXISTS_TAC ‘0’ >> rw [],
+           (* goal 2 (of 2) *)
+           Q.EXISTS_TAC ‘M i’ >> simp [MEM_EL] \\
+           Q.EXISTS_TAC ‘i’ >> rw [] ]) \\
+     Know ‘BT' X (apply p0 (M 0)) r = BT' X (M1 0) r’
+     >- (SIMP_TAC std_ss [Once EQ_SYM_EQ, Abbr ‘M1’] \\
+         MATCH_MP_TAC BT_of_principal_hnf >> simp []) >> Rewr' \\
+     Know ‘BT' X (apply p0 (M i)) r = BT' X (M1 i) r’
+     >- (SIMP_TAC std_ss [Once EQ_SYM_EQ, Abbr ‘M1’] \\
+         MATCH_MP_TAC BT_of_principal_hnf >> simp []) >> Rewr' \\
+     REWRITE_TAC [BT_def] \\
+     NTAC 2 (simp [Once ltree_unfold, BT_generator_def, LMAP_fromList,
+                   ltree_el_def]) \\
+     simp [head_equivalent_def])
+ >> simp [EXT_SKOLEM_THM']
+ >> STRIP_TAC (* this assert f as the children function of all Ms *)
+ >> Q.PAT_X_ASSUM ‘!i. i < k ==> ?y Ns. _’ K_TAC
+ >> Know ‘Ns = f 0’ (* eliminate Ns by f *)
+ >- (POP_ASSUM (MP_TAC o Q.SPEC ‘0’) >> rw [])
+ >> DISCH_THEN (FULL_SIMP_TAC std_ss o wrap)
+ >> ‘!i. i < k ==> solvable (apply p0 (M i))’ by PROVE_TAC []
+ >> Q.PAT_X_ASSUM ‘!i. i < k ==> solvable (apply p0 (M i)) /\ _’ K_TAC
+ >> Know ‘!i. i < k ==> apply p0 (M i) -h->* VAR y @* f i’
+ >- (rpt STRIP_TAC \\
+     Q.PAT_X_ASSUM ‘!i. i < k ==> M1 i = VAR y @* f i /\ _’ drule \\
+     simp [Abbr ‘M1’, principal_hnf_thm'])
+ >> DISCH_TAC
+ (* Now we use ‘h::p IN BT_paths (apply p0 (M i))’ (and ‘M 0’) to show that
+   ‘h < m’, as otherwise p1 (the selector) cannot be properly defined.
+  *)
+ >> Know ‘h < m’
+ >- (Q.PAT_X_ASSUM ‘!i. i < k ==> h::p IN ltree_paths (BT' X (apply p0 (M i)) r)’
+       (MP_TAC o Q.SPEC ‘0’) >> simp [] \\
+     MP_TAC (Q.SPECL [‘X’, ‘apply p0 ((M :num -> term) 0)’, ‘r’ ] BT_paths_thm) \\
+     simp [] >> DISCH_THEN K_TAC \\
+     Know ‘BT' X (apply p0 (M 0)) r = BT' X (M1 0) r’
+     >- (SIMP_TAC std_ss [Once EQ_SYM_EQ, Abbr ‘M1’] \\
+         MATCH_MP_TAC BT_of_principal_hnf >> simp []) >> Rewr' \\
+     Q.PAT_X_ASSUM ‘M1 0 = _’ (REWRITE_TAC o wrap) \\
+     simp [BT_def, Once ltree_unfold, BT_generator_def, LMAP_fromList,
+           ltree_paths_alt_ltree_el, ltree_el_def] \\
+     simp [GSYM BT_def, LNTH_fromList, MAP_MAP_o] \\
+     Cases_on ‘h < m’ >> rw [])
+ >> DISCH_TAC
+ >> Q.PAT_X_ASSUM ‘M1 0 = _’ K_TAC
+ (* p1 is defined as a selector *)
+ >> qabbrev_tac ‘p1 = [[selector h m/y]]’
+ >> ‘Boehm_transform p1’ by rw [Boehm_transform_def, Abbr ‘p1’]
+ >> Know ‘!i. i < k ==> apply (p1 ++ p0) (M i) -h->* EL h (f i)’
+ >- (rw [Boehm_transform_APPEND, Abbr ‘p1’] \\
+     MATCH_MP_TAC hreduce_TRANS \\
+     Q.EXISTS_TAC ‘[selector h m/y] (VAR y @* f i)’ \\
+     CONJ_TAC
+     >- (MATCH_MP_TAC hreduce_substitutive \\
+         Q.PAT_X_ASSUM ‘!i. i < k ==> M1 i = VAR y @* f i /\ _’ drule \\
+         simp [Abbr ‘M1’, principal_hnf_thm']) \\
+     simp [appstar_SUB] \\
+     Know ‘MAP [selector h m/y] (f i) = f i’
+     >- (rw [Once LIST_EQ_REWRITE, EL_MAP] \\
+         MATCH_MP_TAC lemma14b \\
+         Q.PAT_X_ASSUM ‘!i. i < k ==> M1 i = VAR y @* f i /\ _’ drule \\
+         rw [EVERY_MEM] \\
+         POP_ASSUM MATCH_MP_TAC >> rw [EL_MEM]) >> Rewr' \\
+     MATCH_MP_TAC hreduce_selector >> rw [])
+ >> DISCH_TAC
+ (* redefine Ns as the h-subterms of Ms
+
+    NOTE: So far we don't know if any “EL h (f i)” is solvable, thus it's not
+    sure whether “principal_hnf (apply (p1 ++ p0) (M i)) = EL h (f i)”.
+  *)
+ >> qabbrev_tac ‘Ns = GENLIST (EL h o f) k’
+ >> ‘LENGTH Ns = k’ by rw [Abbr ‘Ns’, LENGTH_GENLIST]
+ >> Know ‘!i. i < k ==> MEM (EL h (f i)) Ns’
+ >- (rw [Abbr ‘Ns’, MEM_GENLIST] \\
+     Q.EXISTS_TAC ‘i’ >> art [])
+ >> DISCH_TAC
+ (* proving one antecedent of IH *)
+ >> Know ‘agree_upto X Ns p (SUC r)’
+ >- (fs [agree_upto_def] \\
+     rw [Abbr ‘Ns’, MEM_GENLIST] \\
+     NTAC 2 (POP_ASSUM MP_TAC) \\
+     rename1 ‘a < k ==> b < k ==> _’ >> NTAC 2 STRIP_TAC \\
+     Q.PAT_X_ASSUM ‘!q M N. q <<= h::p /\ q <> h::p /\
+                            MEM M (apply p0 Ms) /\ _ ==> _’
+       (MP_TAC o Q.SPECL [‘h::q’, ‘apply p0 ((M :num -> term) a)’,
+                                  ‘apply p0 ((M :num -> term) b)’]) \\
+     simp [MEM_MAP] \\
+     impl_tac
+     >- (CONJ_TAC >| (* 2 subgoals *)
+         [ (* goal 1 (of 2) *)
+           Q.EXISTS_TAC ‘M a’ >> rw [EL_MEM, Abbr ‘M’],
+           (* goal 2 (of 2) *)
+           Q.EXISTS_TAC ‘M b’ >> rw [EL_MEM, Abbr ‘M’] ]) \\
+     simp [subtree_equiv_def] \\
+     Know ‘BT' X (apply p0 (M a)) r = BT' X (M1 a) r’
+     >- (SIMP_TAC std_ss [Once EQ_SYM_EQ, Abbr ‘M1’] \\
+         MATCH_MP_TAC BT_of_principal_hnf >> simp []) >> Rewr' \\
+     Know ‘BT' X (apply p0 (M b)) r = BT' X (M1 b) r’
+     >- (SIMP_TAC std_ss [Once EQ_SYM_EQ, Abbr ‘M1’] \\
+         MATCH_MP_TAC BT_of_principal_hnf >> simp []) >> Rewr' \\
+     simp [] \\
+    ‘!i. solvable (VAR y @* f i)’ by rw [] \\
+    ‘!i. principal_hnf (VAR y @* f i) = VAR y @* f i’ by rw [] \\
+     Q_TAC (UNBETA_TAC [BT_def, BT_generator_def, Once ltree_unfold,
+                        LMAP_fromList]) ‘BT' X (VAR y @* f a) r’ \\
+     simp [Abbr ‘M0’, GSYM appstar_APPEND, LNTH_fromList, ltree_el_def,
+           GSYM BT_def, Abbr ‘y'’, Abbr ‘Ms'’, Abbr ‘n’, Abbr ‘l’, Abbr ‘M1'’,
+           Abbr ‘vs’, EL_MAP] \\
+     Q_TAC (UNBETA_TAC [BT_def, BT_generator_def, Once ltree_unfold,
+                        LMAP_fromList]) ‘BT' X (VAR y @* f b) r’ \\
+     simp [Abbr ‘M0’, GSYM appstar_APPEND, LNTH_fromList, ltree_el_def,
+           GSYM BT_def, Abbr ‘y'’, Abbr ‘Ms'’, Abbr ‘n’, Abbr ‘l’, Abbr ‘M1'’,
+           Abbr ‘vs’, EL_MAP])
+ >> DISCH_TAC
+ >> qabbrev_tac ‘pi' = p1 ++ p0’
+ >> ‘Boehm_transform pi'’ by rw [Abbr ‘pi'’, Boehm_transform_APPEND]
+ >> Know ‘agree_upto X (apply pi' Ms) p (SUC r)’
+ >- (Q.PAT_X_ASSUM ‘agree_upto X Ns p (SUC r)’ MP_TAC \\
+     rw [agree_upto_def, MEM_MAP, Abbr ‘Ns’, MEM_GENLIST, MEM_EL] \\
+     Know ‘subtree_equiv X (apply pi' (M n)) (apply pi' (M n')) q (SUC r) <=>
+           subtree_equiv X (EL h (f n)) (EL h (f n')) q (SUC r)’
+     >- (MATCH_MP_TAC hreduce_subtree_equiv_cong >> simp []) >> Rewr' \\
+     FIRST_X_ASSUM MATCH_MP_TAC >> rw [] >| (* 2 subgoals *)
+     [ (* goal 1 (of 2) *)
+       Q.EXISTS_TAC ‘n’ >> art [],
+       (* goal 2 (of 2) *)
+       Q.EXISTS_TAC ‘n'’ >> art [] ])
+ >> DISCH_TAC
+ (* proving antecedents of IH *)
+ >> Know ‘!N. MEM N Ns ==> FV N SUBSET X UNION RANK (SUC r)’
+ >- (simp [MEM_EL, Abbr ‘Ns’] \\
+     NTAC 2 STRIP_TAC \\
+     POP_ORW >> simp [EL_GENLIST] \\
+     MATCH_MP_TAC subterm_induction_lemma' \\
+     qexistsl_tac [‘apply p0 (M n)’, ‘M1 n’, ‘0’, ‘m’, ‘[]’, ‘M1 n’] \\
+     simp [])
+ >> DISCH_TAC
+ >> Know ‘!N. MEM N Ns ==> p IN ltree_paths (BT' X N (SUC r))’
+ >- (NTAC 2 STRIP_TAC \\
+     Q.PAT_X_ASSUM ‘!N. MEM N Ns ==> FV N SUBSET X UNION RANK (SUC r)’ drule \\
+     POP_ASSUM MP_TAC \\
+     simp [MEM_EL, Abbr ‘Ns’] \\
+     STRIP_TAC >> POP_ORW \\
+     simp [EL_GENLIST] >> DISCH_TAC \\
+     Q.PAT_X_ASSUM ‘!i. i < k ==> h::p IN ltree_paths (BT' X (apply p0 (M i)) r)’
+       (MP_TAC o Q.SPEC ‘n’) >> simp [] \\
+     MP_TAC (Q.SPECL [‘X’, ‘apply p0 ((M :num -> term) n)’, ‘r’] BT_paths_thm) \\
+     simp [] >> DISCH_THEN K_TAC \\
+     MP_TAC (Q.SPECL [‘X’, ‘EL h (f (n :num))’, ‘SUC r’] BT_paths_thm) \\
+     simp [] >> DISCH_THEN K_TAC \\
+     Know ‘BT' X (apply p0 (M n)) r = BT' X (M1 n) r’
+     >- (SIMP_TAC std_ss [Once EQ_SYM_EQ, Abbr ‘M1’] \\
+         MATCH_MP_TAC BT_of_principal_hnf >> simp []) >> Rewr' \\
+    ‘!i. solvable (VAR y @* f i)’ by rw [] \\
+    ‘!i. principal_hnf (VAR y @* f i) = VAR y @* f i’ by rw [] \\
+     Q_TAC (UNBETA_TAC [BT_def, Once ltree_unfold, BT_generator_def])
+           ‘BT' X (M1 (n :num)) r’ \\
+     simp [LMAP_fromList, ltree_paths_alt_ltree_el, ltree_el_def, GSYM BT_def] \\
+     simp [Abbr ‘M0’, GSYM appstar_APPEND, LNTH_fromList, EL_MAP,
+           Abbr ‘y'’, Abbr ‘Ms'’, Abbr ‘n'’, Abbr ‘l’, Abbr ‘M1'’, Abbr ‘vs’])
+ >> DISCH_TAC
+ >> Know ‘!N. MEM N (apply pi' Ms) ==> p IN ltree_paths (BT' X N (SUC r))’
+ >- (rw [MEM_MAP, MEM_EL] \\
+     Know ‘BT' X (apply pi' (M n)) (SUC r) = BT' X (EL h (f n)) (SUC r)’
+     >- (MATCH_MP_TAC hreduce_BT_cong >> simp []) >> Rewr' \\
+     FIRST_X_ASSUM MATCH_MP_TAC >> simp [])
+ >> DISCH_TAC
+ >> Know ‘!N. MEM N (apply pi' Ms) ==> FV N SUBSET X UNION RANK (SUC r)’
+ >- (rw [MEM_MAP, MEM_EL, Abbr ‘pi'’, Boehm_apply_APPEND, Abbr ‘p1’] \\
+     Q_TAC (TRANS_TAC SUBSET_TRANS) ‘FV (apply p0 (M n))’ \\
+     CONJ_TAC >- (MATCH_MP_TAC FV_SUB_SUBSET >> simp [closed_def]) \\
+     Q_TAC (TRANS_TAC SUBSET_TRANS) ‘X UNION RANK r’ >> simp [] \\
+     Suff ‘RANK r SUBSET RANK (SUC r)’ >- SET_TAC [] \\
+     simp [RANK_MONO])
+ >> DISCH_TAC
+ (* using IH *)
+ >> Q.PAT_X_ASSUM
+      ‘!Ms' r'. Ms' <> [] /\ 0 < r' /\ _ /\ _ /\ agree_upto X Ms' p r' ==>
+               ?pi. Boehm_transform pi /\ faithful p X Ms' pi r'’
+      (MP_TAC o Q.SPECL [‘apply pi' Ms’, ‘SUC r’])
+ >> simp [faithful_def]
+ >> DISCH_THEN (Q.X_CHOOSE_THEN ‘p2’ STRIP_ASSUME_TAC)
+ >> qabbrev_tac ‘pi = p2 ++ p1 ++ p0’
+ >> Q.EXISTS_TAC ‘pi’
+ >> CONJ_TAC (* Boehm_transform pi *)
+ >- (qunabbrev_tac ‘pi’ \\
+     MATCH_MP_TAC Boehm_transform_APPEND >> art [] \\
+     MATCH_MP_TAC Boehm_transform_APPEND >> art [])
+ >> simp [Abbr ‘pi’, GSYM APPEND_ASSOC]
+ >> REWRITE_TAC [Boehm_apply_APPEND]
+ >> Know ‘!i. i < k ==> MEM (apply pi' (M i)) (apply pi' Ms)’
+ >- (rw [MEM_MAP] \\
+     Q.EXISTS_TAC ‘M i’ >> simp [EL_MEM, Abbr ‘M’])
+ >> DISCH_TAC
+ (* stage work, the 2nd part is easier following textbook *)
+ >> reverse CONJ_TAC
+ >- (simp [MEM_EL] \\
+     qx_genl_tac [‘t1’, ‘t2’] (* temporary names, to be consumed soon *) \\
+     ONCE_REWRITE_TAC [TAUT ‘P /\ Q ==> R <=> P ==> Q ==> R’] \\
+     DISCH_THEN (Q.X_CHOOSE_THEN ‘a’ STRIP_ASSUME_TAC) \\
+     DISCH_THEN (Q.X_CHOOSE_THEN ‘b’ STRIP_ASSUME_TAC) \\
+     Q.PAT_X_ASSUM ‘_ = M a’ (ONCE_REWRITE_TAC o wrap) \\
+     Q.PAT_X_ASSUM ‘_ = M b’ (ONCE_REWRITE_TAC o wrap) \\
+     qabbrev_tac ‘t1 = apply pi' (M a)’ \\
+     qabbrev_tac ‘t2 = apply pi' (M b)’ \\
+  (* eliminating “equivalent” *)
+     Q.PAT_X_ASSUM ‘!M N. _ ==> (subtree_equiv X M N p (SUC r) <=>
+                                 equivalent (apply p2 M) (apply p2 N))’
+                   (MP_TAC o ONCE_REWRITE_RULE [EQ_SYM_EQ] o
+                    Q.SPECL [‘t1’, ‘t2’]) \\
+     simp [Abbr ‘t1’, Abbr ‘t2’] >> DISCH_THEN K_TAC \\
+     rpt (Q.PAT_X_ASSUM ‘agree_upto X _ _ _’ K_TAC) \\
+  (* applying hreduce_subtree_equiv_cong *)
+     Know ‘subtree_equiv X (apply p0 (M a)) (apply p0 (M b)) (h::p) r <=>
+           subtree_equiv X (VAR y @* f a) (VAR y @* f b) (h::p) r’
+     >- (MATCH_MP_TAC hreduce_subtree_equiv_cong >> simp []) >> Rewr' \\
+     Know ‘subtree_equiv X (apply pi' (M a)) (apply pi' (M b)) p (SUC r) <=>
+           subtree_equiv X (EL h (f a)) (EL h (f b)) p (SUC r)’
+     >- (MATCH_MP_TAC hreduce_subtree_equiv_cong >> simp []) >> Rewr' \\
+     simp [subtree_equiv_def] \\
+    ‘!i. solvable (VAR y @* f i)’ by rw [] \\
+    ‘!i. principal_hnf (VAR y @* f i) = VAR y @* f i’ by rw [] \\
+     Q_TAC (UNBETA_TAC [BT_def, BT_generator_def, Once ltree_unfold,
+                        LMAP_fromList, LET_DEF]) ‘BT' X (VAR y @* f a) r’ \\
+     simp [GSYM BT_def, LMAP_fromList, ltree_el_def, LNTH_fromList, EL_MAP] \\
+     Q_TAC (UNBETA_TAC [BT_def, BT_generator_def, Once ltree_unfold,
+                        LMAP_fromList, LET_DEF]) ‘BT' X (VAR y @* f b) r’ \\
+     simp [GSYM BT_def, LMAP_fromList, ltree_el_def, LNTH_fromList, EL_MAP])
+ (* final goal *)
+ >> rpt STRIP_TAC
+ (* clean up all assumptions involving term equivalences *)
+ >> rpt (Q.PAT_X_ASSUM ‘agree_upto X _ _ _’ K_TAC)
+ >> qabbrev_tac ‘N = apply pi' (M i)’
+ >> Q.PAT_X_ASSUM ‘!M. MEM M (apply pi' Ms) ==>
+                      (p IN BT_valid_paths M <=> solvable (apply p2 M))’
+                  (MP_TAC o ONCE_REWRITE_RULE [EQ_SYM_EQ] o Q.SPEC ‘N’)
+ >> simp [Abbr ‘N’]
+ >> DISCH_THEN K_TAC
+ >> qabbrev_tac ‘N = apply pi' (M i)’
+ (* applying BT_valid_paths_thm' to turn the goal to subterm arguments *)
+ >> Know ‘BT_valid_paths N = {p | subterm X N p (SUC r) <> NONE /\
+                                  solvable (subterm' X N p (SUC r))}’
+ >- (MATCH_MP_TAC BT_valid_paths_thm' >> simp [Abbr ‘N’])
+ >> Rewr'
+ >> Know ‘BT_valid_paths (M i) = {p | subterm X (M i) p r <> NONE /\
+                                      solvable (subterm' X (M i) p r)}’
+ >- (MATCH_MP_TAC BT_valid_paths_thm' >> simp [])
+ >> Rewr'
+ >> simp [Abbr ‘N’]
+ (* applying BT_ltree_paths_thm *)
+ >> ‘subterm X (M i) (h::p) r <> NONE’ by simp [GSYM BT_ltree_paths_thm]
+ >> ‘subterm X (apply pi' (M i)) p (SUC r) <> NONE’
+      by simp [GSYM BT_ltree_paths_thm]
+ >> simp []
+ (* applying hreduce_subterm_cong *)
+ >> Know ‘subterm X (apply p0 (M i)) (h::p) r =
+          subterm X (VAR y @* f i) (h::p) r’
+ >- (MATCH_MP_TAC hreduce_subterm_cong >> simp [])
+ >> Rewr'
+ (* NOTE: To apply hreduce_subterm_cong to “subterm' X (apply pi' (M i)”,
+   ‘p <> []’ is required. The case ‘p = []’ is trivial.
+  *)
+ >> Cases_on ‘p = []’
+ >- (simp [] \\
+     Know ‘solvable (apply pi' (M i)) <=> solvable (EL h (f i))’
+     >- (MATCH_MP_TAC hreduce_solvable_cong >> simp []) >> Rewr' \\
+     Suff ‘subterm' X (VAR y @* f i) [h] r = EL h (f i)’ >- rw [] \\
+     rw [subterm_def])
+ >> Know ‘subterm X (apply pi' (M i)) p (SUC r) =
+          subterm X (EL h (f i)) p (SUC r)’
+ >- (MATCH_MP_TAC hreduce_subterm_cong >> simp [])
+ >> Rewr'
+ >> Suff ‘subterm' X (VAR y @* f i) (h::p) r =
+          subterm' X (EL h (f i)) p (SUC r)’ >- rw []
+ >> ‘!i. solvable (VAR y @* f i)’ by rw []
+ >> ‘!i. principal_hnf (VAR y @* f i) = VAR y @* f i’ by rw []
+ >> Q_TAC (UNBETA_TAC [subterm_def]) ‘subterm X (VAR y @* f i) (h::p) r’
+ >> simp []
+ *)
 QED
 
 (* END *)
